heap_lang/lib/barrier/proof.v
@@ -162,7 +162,7 @@ Proof.
 Qed.
 
 Lemma recv_split E l P1 P2 :
-  nclose N ⊆ E → recv l (P1 ★ P2) ={E}=> recv l P1 ★ recv l P2.
+  nclose N ⊆ E → recv l (P1 ★ P2) ={E}=★ recv l P1 ★ recv l P2.
 Proof.
   rename P1 into R1; rename P2 into R2. rewrite {1}/recv /barrier_ctx.
   iIntros (?). iDestruct 1 as (γ P Q i) "(#(%&Hh&Hsts)&Hγ&#HQ&HQR)".
