program_logic/fancy_updates.v
@@ -6,7 +6,7 @@ Import uPred.
 
 Program Definition fupd_def `{irisG Λ Σ}
     (E1 E2 : coPset) (P : iProp Σ) : iProp Σ :=
-  (wsat ★ ownE E1 =r=★ ◇ (wsat ★ ownE E2 ★ P))%I.
+  (wsat ★ ownE E1 ==★ ◇ (wsat ★ ownE E2 ★ P))%I.
 Definition fupd_aux : { x | x = @fupd_def }. by eexists. Qed.
 Definition fupd := proj1_sig fupd_aux.
 Definition fupd_eq : @fupd = @fupd_def := proj2_sig fupd_aux.
@@ -19,7 +19,7 @@ Notation "|={ E1 , E2 }=> Q" := (fupd E1 E2 Q)
 Notation "P ={ E1 , E2 }=★ Q" := (P -★ |={E1,E2}=> Q)%I
   (at level 99, E1,E2 at level 50, Q at level 200,
    format "P  ={ E1 , E2 }=★  Q") : uPred_scope.
-Notation "P ={ E1 , E2 }=> Q" := (P ⊢ |={E1,E2}=> Q)
+Notation "P ={ E1 , E2 }=★ Q" := (P ⊢ |={E1,E2}=> Q)
   (at level 99, E1, E2 at level 50, Q at level 200, only parsing) : C_scope.
 
 Notation "|={ E }=> Q" := (fupd E E Q)
@@ -28,7 +28,7 @@ Notation "|={ E }=> Q" := (fupd E E Q)
 Notation "P ={ E }=★ Q" := (P -★ |={E}=> Q)%I
   (at level 99, E at level 50, Q at level 200,
    format "P  ={ E }=★  Q") : uPred_scope.
-Notation "P ={ E }=> Q" := (P ⊢ |={E}=> Q)
+Notation "P ={ E }=★ Q" := (P ⊢ |={E}=> Q)
   (at level 99, E at level 50, Q at level 200, only parsing) : C_scope.
 
 Notation "|={ E1 , E2 }▷=> Q" := (|={E1,E2}=> (▷ |={E2,E1}=> Q))%I
@@ -55,31 +55,31 @@ Proof.
   by iFrame.
 Qed.
 
-Lemma except_last_fupd E1 E2 P : ◇ (|={E1,E2}=> P) ={E1,E2}=> P.
+Lemma except_last_fupd E1 E2 P : ◇ (|={E1,E2}=> P) ={E1,E2}=★ P.
 Proof.
   rewrite fupd_eq. iIntros "H [Hw HE]". iTimeless "H". iApply "H"; by iFrame.
 Qed.
 
-Lemma bupd_fupd E P : (|=r=> P) ={E}=> P.
+Lemma bupd_fupd E P : (|==> P) ={E}=★ P.
 Proof.
   rewrite fupd_eq /fupd_def. iIntros "H [$ $]"; iUpd "H".
   iUpdIntro. by iApply except_last_intro.
 Qed.
 
-Lemma fupd_mono E1 E2 P Q : (P ⊢ Q) → (|={E1,E2}=> P) ={E1,E2}=> Q.
+Lemma fupd_mono E1 E2 P Q : (P ⊢ Q) → (|={E1,E2}=> P) ={E1,E2}=★ Q.
 Proof.
   rewrite fupd_eq /fupd_def. iIntros (HPQ) "HP HwE".
   rewrite -HPQ. by iApply "HP".
 Qed.
 
-Lemma fupd_trans E1 E2 E3 P : (|={E1,E2}=> |={E2,E3}=> P) ={E1,E3}=> P.
+Lemma fupd_trans E1 E2 E3 P : (|={E1,E2}=> |={E2,E3}=> P) ={E1,E3}=★ P.
 Proof.
   rewrite fupd_eq /fupd_def. iIntros "HP HwE".
   iUpd ("HP" with "HwE") as ">(Hw & HE & HP)". iApply "HP"; by iFrame.
 Qed.
 
 Lemma fupd_mask_frame_r' E1 E2 Ef P :
-  E1 ⊥ Ef → (|={E1,E2}=> E2 ⊥ Ef → P) ={E1 ∪ Ef,E2 ∪ Ef}=> P.
+  E1 ⊥ Ef → (|={E1,E2}=> E2 ⊥ Ef → P) ={E1 ∪ Ef,E2 ∪ Ef}=★ P.
 Proof.
   intros. rewrite fupd_eq /fupd_def ownE_op //. iIntros "Hvs (Hw & HE1 &HEf)".
   iUpd ("Hvs" with "[Hw HE1]") as ">($ & HE2 & HP)"; first by iFrame.
@@ -87,7 +87,7 @@ Proof.
   iUpdIntro; iApply except_last_intro. by iApply "HP".
 Qed.
 
-Lemma fupd_frame_r E1 E2 P Q : (|={E1,E2}=> P) ★ Q ={E1,E2}=> P ★ Q.
+Lemma fupd_frame_r E1 E2 P Q : (|={E1,E2}=> P) ★ Q ={E1,E2}=★ P ★ Q.
 Proof. rewrite fupd_eq /fupd_def. by iIntros "[HwP $]". Qed.
 
 (** * Derived rules *)
@@ -97,50 +97,50 @@ Global Instance fupd_flip_mono' E1 E2 :
   Proper (flip (⊢) ==> flip (⊢)) (@fupd Λ Σ _ E1 E2).
 Proof. intros P Q; apply fupd_mono. Qed.
 
-Lemma fupd_intro E P : P ={E}=> P.
+Lemma fupd_intro E P : P ={E}=★ P.
 Proof. iIntros "HP". by iApply bupd_fupd. Qed.
 Lemma fupd_intro_mask' E1 E2 : E2 ⊆ E1 → True ⊢ |={E1,E2}=> |={E2,E1}=> True.
 Proof. exact: fupd_intro_mask. Qed.
-Lemma fupd_except_last E1 E2 P : (|={E1,E2}=> ◇ P) ={E1,E2}=> P.
+Lemma fupd_except_last E1 E2 P : (|={E1,E2}=> ◇ P) ={E1,E2}=★ P.
 Proof. by rewrite {1}(fupd_intro E2 P) except_last_fupd fupd_trans. Qed.
 
-Lemma fupd_frame_l E1 E2 P Q : (P ★ |={E1,E2}=> Q) ={E1,E2}=> P ★ Q.
+Lemma fupd_frame_l E1 E2 P Q : (P ★ |={E1,E2}=> Q) ={E1,E2}=★ P ★ Q.
 Proof. rewrite !(comm _ P); apply fupd_frame_r. Qed.
-Lemma fupd_wand_l E1 E2 P Q : (P -★ Q) ★ (|={E1,E2}=> P) ={E1,E2}=> Q.
+Lemma fupd_wand_l E1 E2 P Q : (P -★ Q) ★ (|={E1,E2}=> P) ={E1,E2}=★ Q.
 Proof. by rewrite fupd_frame_l wand_elim_l. Qed.
-Lemma fupd_wand_r E1 E2 P Q : (|={E1,E2}=> P) ★ (P -★ Q) ={E1,E2}=> Q.
+Lemma fupd_wand_r E1 E2 P Q : (|={E1,E2}=> P) ★ (P -★ Q) ={E1,E2}=★ Q.
 Proof. by rewrite fupd_frame_r wand_elim_r. Qed.
 
 Lemma fupd_trans_frame E1 E2 E3 P Q :
-  ((Q ={E2,E3}=★ True) ★ |={E1,E2}=> (Q ★ P)) ={E1,E3}=> P.
+  ((Q ={E2,E3}=★ True) ★ |={E1,E2}=> (Q ★ P)) ={E1,E3}=★ P.
 Proof.
   rewrite fupd_frame_l assoc -(comm _ Q) wand_elim_r.
   by rewrite fupd_frame_r left_id fupd_trans.
 Qed.
 
 Lemma fupd_mask_frame_r E1 E2 Ef P :
-  E1 ⊥ Ef → (|={E1,E2}=> P) ={E1 ∪ Ef,E2 ∪ Ef}=> P.
+  E1 ⊥ Ef → (|={E1,E2}=> P) ={E1 ∪ Ef,E2 ∪ Ef}=★ P.
 Proof.
   iIntros (?) "H". iApply fupd_mask_frame_r'; auto.
   iApply fupd_wand_r; iFrame "H"; eauto.
 Qed.
-Lemma fupd_mask_mono E1 E2 P : E1 ⊆ E2 → (|={E1}=> P) ={E2}=> P.
+Lemma fupd_mask_mono E1 E2 P : E1 ⊆ E2 → (|={E1}=> P) ={E2}=★ P.
 Proof.
   intros (Ef&->&?)%subseteq_disjoint_union_L. by apply fupd_mask_frame_r.
 Qed.
 
-Lemma fupd_sep E P Q : (|={E}=> P) ★ (|={E}=> Q) ={E}=> P ★ Q.
+Lemma fupd_sep E P Q : (|={E}=> P) ★ (|={E}=> Q) ={E}=★ P ★ Q.
 Proof. by rewrite fupd_frame_r fupd_frame_l fupd_trans. Qed.
 Lemma fupd_big_sepM `{Countable K} {A} E (Φ : K → A → iProp Σ) (m : gmap K A) :
-  ([★ map] k↦x ∈ m, |={E}=> Φ k x) ={E}=> [★ map] k↦x ∈ m, Φ k x.
+  ([★ map] k↦x ∈ m, |={E}=> Φ k x) ={E}=★ [★ map] k↦x ∈ m, Φ k x.
 Proof.
-  apply (big_opM_forall (λ P Q, P ={E}=> Q)); auto using fupd_intro.
+  apply (big_opM_forall (λ P Q, P ={E}=★ Q)); auto using fupd_intro.
   intros P1 P2 HP Q1 Q2 HQ. by rewrite HP HQ -fupd_sep.
 Qed.
 Lemma fupd_big_sepS `{Countable A} E (Φ : A → iProp Σ) X :
-  ([★ set] x ∈ X, |={E}=> Φ x) ={E}=> [★ set] x ∈ X, Φ x.
+  ([★ set] x ∈ X, |={E}=> Φ x) ={E}=★ [★ set] x ∈ X, Φ x.
 Proof.
-  apply (big_opS_forall (λ P Q, P ={E}=> Q)); auto using fupd_intro.
+  apply (big_opS_forall (λ P Q, P ={E}=★ Q)); auto using fupd_intro.
   intros P1 P2 HP Q1 Q2 HQ. by rewrite HP HQ -fupd_sep.
 Qed.
 End fupd.
@@ -154,7 +154,7 @@ Section proofmode_classes.
   Proof. rewrite /FromPure. intros <-. apply fupd_intro. Qed.
 
   Global Instance from_assumption_fupd E p P Q :
-    FromAssumption p P (|=r=> Q) → FromAssumption p P (|={E}=> Q)%I.
+    FromAssumption p P (|==> Q) → FromAssumption p P (|={E}=> Q)%I.
   Proof. rewrite /FromAssumption=>->. apply bupd_fupd. Qed.
 
   Global Instance into_wand_fupd E1 E2 R P Q :
@@ -186,7 +186,7 @@ Section proofmode_classes.
   Proof. by rewrite /FromUpd -bupd_fupd. Qed.
 
   Global Instance elim_upd_bupd_fupd E1 E2 P Q :
-    ElimUpd (|=r=> P) P (|={E1,E2}=> Q) (|={E1,E2}=> Q).
+    ElimUpd (|==> P) P (|={E1,E2}=> Q) (|={E1,E2}=> Q).
   Proof. by rewrite /ElimUpd (bupd_fupd E1) fupd_frame_r wand_elim_r fupd_trans. Qed.
   Global Instance elim_upd_fupd_fupd E1 E2 E3 P Q :
     ElimUpd (|={E1,E2}=> P) P (|={E1,E3}=> Q) (|={E2,E3}=> Q).
