proofmode/class_instances.v
@@ -16,7 +16,7 @@ Global Instance from_assumption_always_r P Q :
   FromAssumption true P Q → FromAssumption true P (□ Q).
 Proof. rewrite /FromAssumption=><-. by rewrite always_always. Qed.
 Global Instance from_assumption_bupd p P Q :
-  FromAssumption p P Q → FromAssumption p P (|=r=> Q)%I.
+  FromAssumption p P Q → FromAssumption p P (|==> Q)%I.
 Proof. rewrite /FromAssumption=>->. apply bupd_intro. Qed.
 
 (* IntoPure *)
@@ -40,7 +40,7 @@ Proof.
   rewrite /FromPure. eapply pure_elim; [done|]=> ?.
   rewrite -cmra_valid_intro //. auto with I.
 Qed.
-Global Instance from_pure_bupd P φ : FromPure P φ → FromPure (|=r=> P) φ.
+Global Instance from_pure_bupd P φ : FromPure P φ → FromPure (|==> P) φ.
 Proof. rewrite /FromPure=> ->. apply bupd_intro. Qed.
 
 (* IntoPersistentP *)
@@ -110,7 +110,7 @@ Proof. apply and_elim_r', impl_wand. Qed.
 Global Instance into_wand_always R P Q : IntoWand R P Q → IntoWand (□ R) P Q.
 Proof. rewrite /IntoWand=> ->. apply always_elim. Qed.
 Global Instance into_wand_bupd R P Q :
-  IntoWand R P Q → IntoWand R (|=r=> P) (|=r=> Q) | 100.
+  IntoWand R P Q → IntoWand R (|==> P) (|==> Q) | 100.
 Proof. rewrite /IntoWand=>->. apply wand_intro_l. by rewrite bupd_wand_r. Qed.
 
 (* FromAnd *)
@@ -143,7 +143,7 @@ Global Instance from_sep_later P Q1 Q2 :
   FromSep P Q1 Q2 → FromSep (▷ P) (▷ Q1) (▷ Q2).
 Proof. rewrite /FromSep=> <-. by rewrite later_sep. Qed.
 Global Instance from_sep_bupd P Q1 Q2 :
-  FromSep P Q1 Q2 → FromSep (|=r=> P) (|=r=> Q1) (|=r=> Q2).
+  FromSep P Q1 Q2 → FromSep (|==> P) (|==> Q1) (|==> Q2).
 Proof. rewrite /FromSep=><-. apply bupd_sep. Qed.
 
 Global Instance from_sep_big_sepM
@@ -317,14 +317,14 @@ Global Instance frame_forall {A} R (Φ Ψ : A → uPred M) :
   (∀ a, Frame R (Φ a) (Ψ a)) → Frame R (∀ x, Φ x) (∀ x, Ψ x).
 Proof. rewrite /Frame=> ?. by rewrite sep_forall_l; apply forall_mono. Qed.
 
-Global Instance frame_bupd R P Q : Frame R P Q → Frame R (|=r=> P) (|=r=> Q).
+Global Instance frame_bupd R P Q : Frame R P Q → Frame R (|==> P) (|==> Q).
 Proof. rewrite /Frame=><-. by rewrite bupd_frame_l. Qed.
 
 (* FromOr *)
 Global Instance from_or_or P1 P2 : FromOr (P1 ∨ P2) P1 P2.
 Proof. done. Qed.
 Global Instance from_or_bupd P Q1 Q2 :
-  FromOr P Q1 Q2 → FromOr (|=r=> P) (|=r=> Q1) (|=r=> Q2).
+  FromOr P Q1 Q2 → FromOr (|==> P) (|==> Q1) (|==> Q2).
 Proof. rewrite /FromOr=><-. apply or_elim; apply bupd_mono; auto with I. Qed.
 
 (* IntoOr *)
@@ -338,7 +338,7 @@ Proof. rewrite /IntoOr=>->. by rewrite later_or. Qed.
 Global Instance from_exist_exist {A} (Φ : A → uPred M): FromExist (∃ a, Φ a) Φ.
 Proof. done. Qed.
 Global Instance from_exist_bupd {A} P (Φ : A → uPred M) :
-  FromExist P Φ → FromExist (|=r=> P) (λ a, |=r=> Φ a)%I.
+  FromExist P Φ → FromExist (|==> P) (λ a, |==> Φ a)%I.
 Proof.
   rewrite /FromExist=><-. apply exist_elim=> a. by rewrite -(exist_intro a).
 Qed.
@@ -367,17 +367,17 @@ Global Instance is_except_last_except_last P : IsExceptLast (◇ P).
 Proof. by rewrite /IsExceptLast except_last_idemp. Qed.
 Global Instance is_except_last_later P : IsExceptLast (▷ P).
 Proof. by rewrite /IsExceptLast except_last_later. Qed.
-Global Instance is_except_last_bupd P : IsExceptLast P → IsExceptLast (|=r=> P).
+Global Instance is_except_last_bupd P : IsExceptLast P → IsExceptLast (|==> P).
 Proof.
   rewrite /IsExceptLast=> HP.
   by rewrite -{2}HP -(except_last_idemp P) -except_last_bupd -(except_last_intro P).
 Qed.
 
 (* FromUpd *)
-Global Instance from_upd_bupd P : FromUpd (|=r=> P) P.
+Global Instance from_upd_bupd P : FromUpd (|==> P) P.
 Proof. done. Qed.
 
 (* ElimVs *)
-Global Instance elim_upd_bupd_bupd P Q : ElimUpd (|=r=> P) P (|=r=> Q) (|=r=> Q).
+Global Instance elim_upd_bupd_bupd P Q : ElimUpd (|==> P) P (|==> Q) (|==> Q).
 Proof. by rewrite /ElimUpd bupd_frame_r wand_elim_r bupd_trans. Qed.
 End classes.
